src/iteration.v
@@ -11,71 +11,82 @@ Set Universe Polymorphism.
 
 Section Iter.
 
-(* We distinguish the state of the producer and the state of the user.
+(* We distinguish the producer state and the user state.
 
-   For example, the state of the producer could be an integer index,
-   a list of elements that have been enumerated, or a list of
-   elements that remain to be enumerated.
+   For example, the state of the producer could be an integer index, a list
+   of elements that have been enumerated, or a list of elements that remain
+   to be enumerated.
 
-   The type of the user state is whatever the user chooses.
-   The user state is also known as the accumulator,
-   or the loop-carried state. *)
+   The type of the user state is whatever the user chooses. The user state
+   is also known as the accumulator, or the loop-carried state. *)
 
-(* [I] and [N] are the physical and logical types of the producer's
-   state. In a loop over machine integers, the producer's state is
-   the loop index, so these types are [int] and [nat]. *)
-Context {I N : Type}.
+(* [P] is the type of the producer state. *)
+Context {P : Type}.
+Implicit Types i j k : P.
 
 (* [S] is the type of the user's state. *)
 Context {S : Type}.
+Implicit Types s : S.
 
-(* The relation [step] describes the evolution of the producer's state
-   and the manner in which this evolution is observed by the user.
-   The proposition [step j0 _j j j1] means that, in one loop iteration,
-   the producer's state can evolve from [j0] to [j1], while the user
-   (that is, the loop body) observes the current physical index [_j]
-   and logical index [j]. *)
-Variable step : N → I → N → N → Prop.
+(* [O] is the type of the observations delivered by the producer to the
+   user. For example, in a loop over machine integers, this type could be
+   [int]. In a loop over a collection, it could be the type of elements. *)
+Context {O : Type}.
+Implicit Type o : O.
 
-(* The body of the loop is abstracted as a [wp] judgement. The proposition
-   [body _j j s Q] means that the loop body, with current physical index
-   [_j], current logical index [j], and current state [s], establishes the
-   postcondition [Q]. *)
-Variable body : I → N → S → (S → Prop) → Prop.
+(* The relation [step] describes the evolution of the producer's state and
+   the manner in which this evolution is observed by the user. The
+   proposition [step j0 o j j1] means that, in one loop iteration, the
+   producer's state can evolve from [j0] to [j1], while the user (that is,
+   the loop body) observes the observation [o] and producer state [j].
 
-(* In [step] and [body], one could package up [_j] and [j] as a pair of type
-   [I * N] and, abstract this type as a type [O] of user observations. That
-   would be perhaps more pleasing in principle; in practice, the curried
-   form seems more convenient. *)
+   The current producer state [j] is typically either [j0] or [j1].
+   Parameterizing [step] and [body] (below) with [o] and [j] rather than
+   just [o] seems convenient. *)
+Variable step : P → O → P → P → Prop.
 
-(* The loop is abstracted as a [wp] judgement. The proposition [loop s Q]
-   means that the loop, applied to the initial state [s], establishes the
-   postcondition [Q]. *)
+(* The behavior of the loop body is represented by [body], a [wp]-like
+   judgement. The proposition [body o j s Q] means that the loop body, with
+   observation [o], current producer state [j], and current user state [s],
+   establishes the postcondition [Q]. *)
+Variable body : O → P → S → (S → Prop) → Prop.
+
+(* The behavior of the whole loop is represented by [loop], a [wp]-like
+   judgement. The proposition [loop s Q] means that the loop, applied to the
+   initial state [s], establishes the postcondition [Q]. *)
 Variable loop : S → (S → Prop) → Prop.
 
 (* The user's loop invariant takes the form [inv i s], where [i] is the
    current logical producer state and [s] is the current user state. *)
 
-(* In the specification [ITER i k],
-   [i] and [k] are the initial and final producer states. *)
+Implicit Types inv : P → S → Prop.
+
+(* [i] and [k] are the initial and final producer states. *)
+
+(* Then, the specification of a loop takes the following form. *)
 
 Definition ITER i k :=
-  ∀ (inv : N → S → Prop) (s : S),
-  (* The invariant must hold of the initial producer state [i] and
-     initial user state [s]. *)
+  ∀ inv s ,
+  (* Initially, the producer state is [i] and the user state is [s].
+     The invariant must hold. *)
   inv i s →
-  (* If the producer can step from [j0] to [j1] while producing the
-     observable data [_j] and [j], then the loop body, applied to
-     [_j] and [j], must transform [inv j0 s] into [inv j1 s']. *)
-  (∀ j0 _j j j1 s ,
-    step j0 _j j j1 →
+  (* If the producer can step from [j0] to [j1] while revealing the
+     observation [o] and current state [j], then the loop body,
+     applied to [o] and [j], must transform [inv j0 s] into
+     [inv j1 s']. *)
+  (∀ j0 o j j1 s ,
+    step j0 o j j1 →
     inv j0 s →
-    body _j j s (λ s', inv j1 s')
+    body o j s (λ s', inv j1 s')
   ) →
-  (* Once the loop ends, the invariant holds of the final producer state [k]
-     and of the final user state [s]. *)
-  ∀ Q,
+  (* Once the loop ends, the producer state is [k] and the user state is
+     some state [s]. Then, the invariant is guaranteed to hold. *)
+  ∀ Q ,
   (∀ s, inv k s → Q s) →
   loop s Q.
 
 End Iter.
+
+Ltac ITER :=
+  unfold ITER;
+  intros ? ? Hinit Hstep ? Hfinish.
